src/SynthesisFacts.v
@@ -227,14 +227,32 @@ Proof.
   simpl; rewrite IHrb; reflexivity.
 Qed.
 
+Lemma SimMP_int_msg_begin:
+  forall (mp: Msg -> Msg) imsgs smsgs,
+    SimMP mp imsgs smsgs ->
+    forall from to chn rqin,
+      firstMP from to chn imsgs = Some {| tmsg_msg := rqin; tmsg_info := None |} ->
+      forall tid,
+        ForallMP (fun tmsg =>
+                    match tmsg_info tmsg with
+                    | Some ti => tinfo_tid ti < tid
+                    | None => True
+                    end) imsgs ->
+        forall mouts,
+          mouts <> nil ->
+          Forall (fun tmsg => tmsg_info tmsg = Some {| tinfo_tid := tid; tinfo_rqin := rqin |}) mouts ->
+          SimMP mp (distributeMsgs mouts (deqMP from to chn imsgs)) smsgs.
+Proof.
+Admitted.
+
 Lemma SimMP_int_msg_fwd:
   forall (mp: Msg -> Msg) imsgs smsgs,
     SimMP mp imsgs smsgs ->
-    forall from to chn imsg tinfo,
-      firstMP from to chn imsgs = Some {| tmsg_msg := imsg; tmsg_info := Some tinfo |} ->
+    forall from to chn imsg ti,
+      firstMP from to chn imsgs = Some {| tmsg_msg := imsg; tmsg_info := Some ti |} ->
       forall mouts,
         mouts <> nil ->
-        Forall (fun tmsg => tmsg_info tmsg = Some tinfo) mouts ->
+        Forall (fun tmsg => tmsg_info tmsg = Some ti) mouts ->
         SimMP mp (distributeMsgs mouts (deqMP from to chn imsgs)) smsgs.
 Proof.
 Admitted.
